simulate fixpoint kinding of rec in refreshing by lowering kind flag to no refs

theories/typing.v
@@ -1264,6 +1264,13 @@ Definition mk_ser_kind (κ : kind) : kind :=
   | MEMTYPE σ ξ => MEMTYPE σ ξ
   end.
 
+Definition lower_kind_flag_to_no_refs κ : kind :=
+  match κ with
+  | VALTYPE ρ _ => VALTYPE ρ NoRefs
+  | MEMTYPE σ _ => MEMTYPE σ NoRefs
+  end.
+
+
 Inductive refreshed_kinds : function_ctx → type → type → Prop :=
 | RKVar F t : refreshed_kinds F (VarT t) (VarT t)
 | RKI31 F κ : refreshed_kinds F (I31T κ) (I31T (VALTYPE (AtomR PtrR) NoRefs))
@@ -1302,10 +1309,10 @@ Inductive refreshed_kinds : function_ctx → type → type → Prop :=
   refreshed_kinds F (PlugT κ ρ) (PlugT (VALTYPE ρ NoRefs) ρ)
 | RKSpan F κ σ :
   refreshed_kinds F (SpanT κ σ) (SpanT (MEMTYPE σ NoRefs) σ)
-| RKRec F κ τ τ' :
-  refreshed_kinds (F <| fc_type_vars ::= cons κ |>) τ τ' →
-  (* type_kind (fc_type_vars F) τ' = Some κ' -> *)
-  refreshed_kinds F (RecT κ τ) (RecT κ τ') (* does the κ here need to be adjusted..? *)
+| RKRec F κ κ' τ τ' :
+  refreshed_kinds (F <| fc_type_vars ::= cons (lower_kind_flag_to_no_refs κ) |>) τ τ' →
+  type_kind (fc_type_vars F) τ' = Some κ' ->
+  refreshed_kinds F (RecT κ τ) (RecT κ' τ') (* does the κ here need to be adjusted..? *)
 | RKExistsMem F κ κ' τ τ' :
   refreshed_kinds (F <| fc_kind_ctx ::= set kc_mem_vars S |>) τ τ' →
   type_kind (fc_type_vars ((F <| fc_kind_ctx ::= set kc_mem_vars S |>))) τ' = Some κ' ->
