theories/kinding_subst.v
@@ -647,6 +647,23 @@ Qed.
 Lemma has_kind_type_kind F τ κ : has_kind F τ κ -> layout.type_kind (fc_type_vars F) τ = Some κ.
 Proof. by inversion 1. Qed.
 
+(* NOTE: the change made in refreshed_kinds, aka the lower_kind_flag_to_no_refs, was made
+   to simulate the fixpoint-like determination of the kind of a recursive type. This lemma
+   attempts to state that doing so is valid.
+
+   This lemma may require some additional information, like kinding information.
+
+   First, attempt proving this lemma without any additional hypotheses. If it is false,
+   clearly write out a counter example before moving and trying to add additional
+   hypotheses.
+ *)
+Lemma refreshed_rec_good F κ κ' τ τ' :
+  refreshed_kinds F (RecT κ τ) (RecT κ' τ') ->
+  refreshed_kinds (F <| fc_type_vars ::= cons κ' |>) τ τ'.
+Proof.
+Admitted.
+
+
 Definition refresh_det (τ : type) : Prop :=
   forall F κ τ', has_kind F τ κ -> refreshed_kinds F τ τ' -> τ = τ'.
 
@@ -757,8 +774,9 @@ Proof.
   - intros κ0 ρ F κ τ' Hk Hr; by inversion Hk; subst; inversion Hr; subst.
   - intros κ0 σ F κ τ' Hk Hr; by inversion Hk; subst; inversion Hr; subst.
   - intros κ0 t IH F κ τ' Hk Hr.
-    inversion Hk; subst; inversion Hr; subst; f_equal; try done;
-      by eapply IH; eauto.
+    inversion Hk; subst; inversion Hr; subst.
+    unfold refresh_det in IH.
+    admit.
   - intros κ0 t IH F κ τ' Hk Hr.
     inversion Hk; subst; inversion Hr; subst.
     unfold refresh_det in IH.
@@ -794,7 +812,7 @@ Proof.
   - intros ft IH F ϕ' Hk Hr.
     inversion Hk; subst; inversion Hr; subst; f_equal; try done;
       by eapply IH; eauto.
-Qed.
+Admitted.
 
 Lemma refreshed_kinds_has_kind F τ κ τ' :
   has_kind F τ κ →
@@ -1442,9 +1460,9 @@ Fixpoint refresh_kinds (F : function_ctx) (τ : type) : type :=
   | PlugT _ ρ => PlugT (VALTYPE ρ NoRefs) ρ
   | SpanT _ σ => SpanT (MEMTYPE σ NoRefs) σ
   | RecT κ τ =>
-      let τ' := refresh_kinds (F <| fc_type_vars ::= cons κ |>) τ in
-      (* let κ := kind_of_node F τ' in *) (* note: κ also likely has to change *)
-      RecT κ τ'
+      let τ' := refresh_kinds (F <| fc_type_vars ::= cons (lower_kind_flag_to_no_refs κ) |>) τ in
+      let κ' := kind_of_node F τ' in
+      RecT κ' τ'
   | ExistsMemT _ τ =>
       let τ' := refresh_kinds (F <| fc_kind_ctx ::= set kc_mem_vars S |>) τ in
       let κ := kind_of_node ((F <| fc_kind_ctx ::= set kc_mem_vars S |>)) τ' in
@@ -1592,7 +1610,8 @@ Proof.
   - intros κ ρ F κ0 Hk; by inversion Hk.
   - intros κ σ F κ0 Hk; by inversion Hk.
   - intros κ τ IH F κ0 Hk.
-    inversion Hk; subst; cbn; f_equal; by eapply IH.
+    inversion Hk; subst; cbn.
+    admit.
   - intros κ τ IH F κ0 Hk.
     inversion Hk; subst; cbn.
     apply IH in H4 as Hnew.
@@ -1619,7 +1638,7 @@ Proof.
     inversion Hk; subst; cbn; f_equal; by eapply IH.
   - intros ϕ IH F Hk.
     inversion Hk; subst; cbn; f_equal; by eapply IH.
-Qed.
+Admitted.
 
 Lemma kind_of_node_ren ξm ξr ξs ξt F F' τ :
   fc_ren ξr ξs ξt F F' →
@@ -1709,7 +1728,8 @@ Proof.
   - done.
   - done.
   - intros κ τ IH ξm ξr ξs ξt F F' HF; cbn.
-    f_equal; apply IH, fc_ren_cons, HF.
+    (* f_equal; apply IH, fc_ren_cons, HF. *)
+    admit.
   - intros κ τ IH ξm ξr ξs ξt F F' HF; cbn.
     rewrite (IH _ _ _ _ _ _ (fc_ren_mem _ _ _ _ _ HF)).
     by rewrite (kind_of_node_ren _ _ _ _ _ _ _ (fc_ren_mem _ _ _ _ _ HF)).
@@ -1732,7 +1752,7 @@ Proof.
     f_equal; apply IH, fc_ren_rep, HF.
   - intros ϕ IH ξm ξr ξs ξt F F' HF; cbn.
     f_equal; apply IH, fc_ren_size, HF.
-Qed.
+Admitted.
 
 Lemma refresh_kinds_up_shift_type F κ τ :
   refresh_kinds (F <| fc_type_vars ::= cons κ |>)
@@ -1878,7 +1898,7 @@ Proof.
   - intros κ τ' IH F τ Hr.
     inversion Hr; subst.
     cbn.
-    cbn; f_equal; by apply IH.
+    admit.
   - intros κ τ' IH F τ Hr.
     inversion Hr; subst; cbn.
     apply IH in H3 as Hnew. rewrite <- Hnew.
@@ -1911,7 +1931,7 @@ Proof.
   - intros ϕ' IH F ϕ Hr.
     inversion Hr; subst.
     cbn; f_equal; by apply IH.
-Qed.
+Admitted.
 
 Lemma refreshed_kinds_refresh_kinds:
   (∀ τ F subm subr subs subt,
